examples/fai/FAI1.v
@@ -1,3 +1,4 @@
+Require Import Coqlib.
 Require Import ITreelib.
 Require Import ImpPrelude.
 Require Import STS.
@@ -17,25 +18,38 @@ Section PROOF.
 
   Context {Σ : GRA.t}.
   Context `{@GRA.inG memRA Σ}.
+  Variable GlobalStb: gname -> option fspec.
 
-  Definition has_n varg n : iProp := (∃ b ofs, ⌜varg = Vptr b ofs⌝ ** OwnM((b, ofs) |-> [Vint n]))%I.
+  Definition fai_pre b ofs v : Any.t -> Any.t -> iProp :=
+    fun larg harg => 
+      (⌜larg = ([Vptr b ofs])↑ /\ larg = harg⌝ ** OwnM((b, ofs) |-> [v]))%I.
+
+  Definition fai_post b ofs v : Any.t -> Any.t -> iProp :=
+    fun lret hret => 
+      (∃ v', OwnM((b, ofs) |-> [v']) ** ⌜vadd v (Vint 1) = Some v' /\ lret = (Vint 0)↑ /\ hret = lret⌝)%I.
+
+  Definition FAI_pre : () -> Any.t -> Any.t -> iProp :=
+    fun _ larg harg => ⌜exists v, larg = v↑ /\ v <> Vint 0 /\ larg = harg⌝%I.
+
+  Definition FAI_post : () -> Any.t -> Any.t -> iProp :=
+    fun _ larg harg => ⌜larg = harg⌝%I.
 
   Definition FAIF: Any.t -> itree Es Any.t :=
     fun varg =>
-      `varg : val <- varg↓?;;
-      trigger Yield;;;
-      σ <- trigger (Take Σ);;
-      n <- trigger (Take Z);;
-      assume (has_n varg n σ);;;
-      trigger (Call "fai" [varg]↑);;;
-      guarantee (has_n varg (n + 1) σ);;;
-      r <- trigger Yield;;
-      Ret r↑
-    .
+      '(ctx, (t, varg)) <- HoareFunArg FAI_pre varg;;
+      (* '(ctx, varg) <- ASSUME FAI_pre varg ε;; *)
+      ` _ : () <- ccallU "_yield" ();;
+      '(b, ofs, v) <- trigger (Take (nat * Z * val));;
+      '(ctx, varg) <- ASSUME (fai_pre b ofs v) varg ctx;;
+      '(ctx, vret) <- interp_hCallE_tgt GlobalStb ord_top (interp_hEs_tgt (trigger hAPC;;; trigger (Choose _))) ctx;;
+      '(ctx, vret) <- ASSERT (fai_post b ofs v) vret ctx;;
+      ` _ : () <- ccallU "_yield" ();;
+      (* '(_, vret) <- ASSERT FAI_post vret ctx;; *)
+      HoareFunRet FAI_post t (ctx, vret).
 
   Definition FAISem: ModSem.t := {|
     ModSem.fnsems := [("FAI", FAIF)];
-    ModSem.init_st := tt↑;
+    ModSem.init_st := Any.pair tt↑ (ε : Σ)↑;
   |}
   .
 
