examples/fai/FAI01proof.v
@@ -22,17 +22,45 @@ Set Implicit Arguments.
 
 Local Open Scope nat_scope.
 
-
-
 Section SIMMODSEM.
 
   Context `{Σ: GRA.t}.
   Context `{@GRA.inG memRA Σ}.
+  Variable GlobalStb : gname -> option fspec.
 
   Let W : Type := Any.t * Any.t.
 
-  Let wf: unit -> W -> Prop := fun _ _ => True.
+  Let wf: _ -> W -> Prop :=
+    @mk_wf _ unit
+           (fun _ _ _ => ⌜True⌝%I)
+  .
 
+  Theorem correct: refines2 [FAI0.FAI] [FAI1.FAI GlobalStb].
+  Proof.
+    eapply adequacy_local2. econs; ss.
+    i. econstructor 1 with (wf:=wf) (le:=top2); et.
+    { ss. }
+    2: { exists tt. econs. eapply to_semantic. et. }
+    econs; ss. init.
+    unfold FAIF, FAI0.FAIF.
+    harg. unfold FAI_pre in ACC. mDesAll. des. clarify.
+    steps.
+
+    do 2 (prep; _step; simpl).
+    destruct (val_dec v (Vint 0)).
+    { admit. }
+    { ss. steps_safe. _force_l. steps_safe. i. steps_safe. i. steps_safe.
+      force_l. unfold has_n in _ASSUME0. apply from_semantic in _ASSUME0.
+      uipropall. 
+       des. clarify.
+      destruct c.
+      3:{ ur in _ASSUME. clarify. }
+      -  exists (Auth.frag (fun _b _ofs => if (dec b _b) && (dec ofs _ofs) then Excl.just (Vint (x + 1)) else f _b _ofs)).
+      update c (H)
+      { admit. }
+      steps_safe. red. eexists. ss.
+      Unshelve. all: ss.
+  Admitted.
   Theorem correct: refines2 [FAI0.FAI] [FAI1.FAI].
   Proof.
     eapply adequacy_local2. econs; ss.
@@ -40,6 +68,8 @@ Section SIMMODSEM.
     { ss. }
     2: { exists tt. ss. }
     econs; ss. init.
+    unfold FAIF, FAI0.FAIF.
+    
   Admitted.
 
 End SIMMODSEM.
