examples/fai/Main1.v
@@ -6,6 +6,8 @@ Require Import Behavior.
 Require Import ModSem.
 Require Import Skeleton.
 Require Import PCM.
+Require Import HoareDef STB.
+Require Import ProofMode.
 
 Set Implicit Arguments.
 
@@ -13,25 +15,46 @@ Set Implicit Arguments.
 
 Section PROOF.
 
-  Definition mainF: Any.t -> itree Es Any.t :=
+  Context {Σ : GRA.t}.
+  Context `{@GRA.inG memRA Σ}.
+
+  Definition mainF: Any.t -> itree (hEs) Any.t :=
     fun _ =>
-      assume True;;;
       trigger Yield;;;
       trigger (Syscall "print_num" [1%Z]↑ top1);;;
       r <- trigger Yield;;
       Ret r↑
     .
 
-  Definition MainSem: ModSem.t := {|
-    ModSem.fnsems := [("main", mainF)];
-    ModSem.init_st := tt↑;
+  Definition main_spec: fspec :=
+    (mk_simple (fun _ : () => (
+                    ord_top,
+                    fun varg => True%I,
+                    fun vret => True%I
+    )))
+    .
+
+  Definition MainStb: list (gname * fspec).
+    eapply (Seal.sealing "stb").
+    apply [("main", main_spec)].
+  Defined.
+
+  Definition MainSbtb: list (gname * fspecbody) :=
+    [("main", mk_specbody main_spec mainF)].
+
+  Definition SMainSem (sk: Sk.t): SModSem.t := {|
+    SModSem.fnsems := MainSbtb;
+    SModSem.initial_mr := ε;
+    SModSem.initial_st := tt↑;
   |}
   .
 
-  Definition Main: Mod.t := {|
-    Mod.get_modsem := fun _ => MainSem;
-    Mod.sk := Sk.unit;
+  Definition SMain: SMod.t := {|
+    SMod.get_modsem := SMainSem;
+    SMod.sk := Sk.unit;
   |}
   .
+
+  Definition Main stb: Mod.t := SMod.to_tgt stb SMain.
 
 End PROOF.
