examples/fai/Sch0.v
@@ -1,0 +1,79 @@
+Require Import Coqlib.
+Require Import ITreelib.
+Require Import ImpPrelude.
+Require Import STS.
+Require Import Behavior.
+Require Import ModSem.
+Require Import Skeleton.
+Require Import PCM.
+
+Set Implicit Arguments.
+Set Typeclasses Depth 5.
+
+
+
+
+Section PROOF.
+  Section BODY.
+    Context {Es: Type -> Type}.
+    Context `{has_evnetE: eventE -< Es}.
+    Context `{has_schE: schE -< Es}.
+    Context `{has_callE: callE -< Es}.
+    Context (sk: Sk.t).
+
+    Definition spawnF: string * val -> itree Es nat :=
+      fun varg =>
+        let '(fn, args) := varg in
+        trigger (Spawn fn args↑).
+
+    Definition yieldF: () -> itree Es () :=
+      fun _ => trigger Yield.
+
+    (* Definition getpidF: (list val) -> itree Es val :=
+      fun varg =>
+        match varg with
+        | [] =>
+            pid <- trigger EventsL.Getpid;;
+            Ret (Vint (Int.repr (Z.of_nat pid)))
+        | _ => triggerUB
+        end.
+    
+    Definition thread_createF: list val -> itree Es val :=
+      fun varg =>
+        match varg with
+        | [Vptr bid ofsid;Vptr bf ofsf;Vptr barg ofsarg] =>
+            '(gsym, gdata) <- (nth_error sk (pred (Pos.to_nat bf)))?;;
+            gd <- (gdata↓)?;;
+            _ <- (match gd with Cgfun fd => Some fd | _ => None end)?;;
+            `v_pid : val <- ccallU "spawn" (gsym, [Vptr barg ofsarg]);;
+            `_ : unit <- ccallU "store" (Mint16signed, Vptr bid ofsid, v_pid);;
+            Ret (Vint Int.zero)
+        | _ => triggerUB
+        end. *)
+
+  End BODY.
+
+
+
+  Definition SchSem (sk : Sk.t) : ModSem.t :=
+    {|
+      ModSem.fnsems := [("_spawn", cfunU spawnF) ; ("_yield", cfunU yieldF)
+      (* ("thread_yield", cfunU yieldF);
+                        ("get_curid", cfunU getpidF); ("thread_create", cfunU (thread_createF sk)) *)
+                        ];
+      ModSem.init_st := tt↑;
+    |}
+  .
+
+  Definition Sch: Mod.t := {|
+    Mod.get_modsem := SchSem;
+    Mod.sk := [];
+    (* [("thread_yield", (Cgfun (Tfunction Tnil tvoid cc_default))↑);
+               ("get_curid", (Cgfun (Tfunction Tnil tint cc_default))↑);
+               ("thread_create", (Cgfun (Tfunction
+                                           (Tcons (tptr tint)
+                                              (Tcons (tptr (Tfunction (Tcons (tptr tvoid) Tnil) (tptr tvoid) cc_default))
+                                                 (Tcons (tptr tvoid) Tnil))) tint cc_default))↑)]; *)
+  |}
+  .
+End PROOF.
