examples/fai/Sch1.v
@@ -1,0 +1,104 @@
+Require Import Coqlib.
+Require Import ITreelib.
+Require Import ImpPrelude.
+Require Import STS.
+Require Import Behavior.
+Require Import ModSem.
+Require Import Skeleton.
+Require Import PCM.
+Require Import HoareDef STB.
+Require Import ProofMode.
+
+Set Implicit Arguments.
+Set Typeclasses Depth 8.
+
+
+
+
+Section PROOF.
+  Section BODY.
+    Context `{Es: Type -> Type}.
+    Context `{has_evnetE: eventE -< Es}.
+    Context `{has_schE: schE -< Es}.
+    Context `{has_callE: callE -< Es}.
+    Context (sk: Sk.t).
+    Context `{Σ : GRA.t}.
+
+    Definition spawnF: string * val -> itree Es nat :=
+      fun varg =>
+        let '(fn, args) := varg in
+        trigger (Spawn fn args↑).
+
+    (* lee: should invariant dependent on input? *)
+    Definition spawn_spec: fspec :=
+      (mk_simple (fun I => (
+                      ord_top,
+                      (fun varg => I),
+                      (fun vret => I)
+      ))).
+
+
+    Definition yieldF: () -> itree Es () :=
+      fun _ => trigger Yield.
+
+    (* lee: should invariant dependent on input? *)
+    Definition yield_spec: fspec :=
+      (mk_simple (fun I => (
+                      ord_top,
+                      (fun varg => I),
+                      (fun vret => I)
+      ))).
+
+    (* Definition getpidF: (list val) -> itree Es val :=
+      fun varg =>
+        match varg with
+        | [] =>
+            pid <- trigger EventsL.Getpid;;
+            Ret (Vint (Int.repr (Z.of_nat pid)))
+        | _ => triggerUB
+        end.
+    
+    Definition thread_createF: list val -> itree Es val :=
+      fun varg =>
+        match varg with
+        | [Vptr bid ofsid;Vptr bf ofsf;Vptr barg ofsarg] =>
+            '(gsym, gdata) <- (nth_error sk (pred (Pos.to_nat bf)))?;;
+            gd <- (gdata↓)?;;
+            _ <- (match gd with Cgfun fd => Some fd | _ => None end)?;;
+            `v_pid : val <- ccallU "spawn" (gsym, [Vptr barg ofsarg]);;
+            `_ : unit <- ccallU "store" (Mint16signed, Vptr bid ofsid, v_pid);;
+            Ret (Vint Int.zero)
+        | _ => triggerUB
+        end. *)
+
+  End BODY.
+
+  Context `{Σ : GRA.t}.
+
+  Definition SchStb: list (gname * fspec).
+    eapply (Seal.sealing "stb").
+    apply [("_spawn", spawn_spec) ; ("_yield", yield_spec)].
+  Defined.
+
+  Definition SchSbtb: list (gname * fspecbody) :=
+    [("_spawn", mk_specbody spawn_spec (cfunU spawnF));
+    ("_yield",   mk_specbody yield_spec (cfunU yieldF))]
+  .
+
+  Definition SSchSem (sk: Sk.t): SModSem.t := {|
+    SModSem.fnsems := SchSbtb;
+    SModSem.initial_mr := ε;
+    SModSem.initial_st := tt↑;
+  |}
+  .
+
+  Definition SSch: SMod.t := {|
+    SMod.get_modsem := SSchSem;
+    SMod.sk := Sk.unit;
+  |}
+  .
+
+  (* lee: should stb be variable? *)
+  Definition Sch: Mod.t := (SMod.to_tgt (fun _ => to_stb [])) SSch.
+
+End PROOF.
